Arm/Memory/Attr.lean
@@ -23,3 +23,20 @@ register_simp_attr memory_omega
 
 -- Simprocs for address normalization
 register_simp_attr address_normalization
+
+register_option simp_mem.omegaTimeoutMs : Nat := {
+  defValue := 1000
+  descr := "maximum amount of time per omega invocation in milliseconds before `simp_mem` times out. `0` for no timeout."
+}
+
+register_option simp_mem.omegaNumIgnoredTimeouts: Nat := {
+  defValue := 0
+  descr := "number of times omega is allowed to timeout before an error is thrown."
+}
+
+
+def getOmegaTimeoutMs [Monad m] [MonadOptions m] : m Nat := do
+  return simp_mem.omegaTimeoutMs.get (← getOptions)
+
+def getOmegaNumIgnoredTimeouts [Monad m] [MonadOptions m] : m Nat := do
+  return simp_mem.omegaNumIgnoredTimeouts.get (← getOptions)
